Add more Lean for Chapter 9

PieLean/PieLean/Chapter9.lean
@@ -14,7 +14,8 @@ namespace Chapter9
 --  (replace target mot base)
 -- is a
 --  (mot to).
-theorem replace {X: Type} {FROM: X} {TO: X} (target: (FROM = TO)) (MOT: X -> Prop) (base: MOT FROM): MOT TO :=
+theorem replace {X: Type} {FROM: X} {TO: X}
+  (target: (FROM = TO)) (MOT: X -> Prop) (base: MOT FROM): MOT TO :=
   -- https://leanprover-community.github.io/mathlib4_docs/Init/Prelude.html#Eq.subst is replace for Lean.
   -- theorem Eq.subst {α : Sort u}  {motive : α → Prop}  {a b : α}
   --   (h₁ : a = b) (h₂ : motive a) : motive b
@@ -58,20 +59,25 @@ theorem same_cons_Explicit_Eq_subst:
   ∀ (t: Type) (x: t) (as: List t) (bs: List t),
   (as = bs) -> (x :: as) = (x :: bs) :=
   λ t x as bs as_eq_bs =>
-    @Eq.subst (List t) (λ xs => (x :: as) = (x :: xs)) as bs as_eq_bs (Eq.refl (x :: as))
+    @Eq.subst (List t)
+      (λ xs => (x :: as) = (x :: xs))
+      as bs
+      as_eq_bs (Eq.refl (x :: as))
 
 theorem same_cons_Implicit_Eq_subst_with_named:
   ∀ (t: Type) (x: t) (as: List t) (bs: List t),
   (as = bs) -> (x :: as) = (x :: bs) :=
   λ _t x as _bs as_eq_bs =>
-    Eq.subst (motive := (λ xs => (x :: as) = (x :: xs))) as_eq_bs (Eq.refl (x :: as))
+    Eq.subst
+      (motive := (λ xs => (x :: as) = (x :: xs)))
+      as_eq_bs (Eq.refl (x :: as))
 
 theorem same_cons_rewrite_same:
   ∀ (t: Type) (x: t) (as: List t) (bs: List t),
   (as = bs) -> (x :: as) = (x :: bs) := by
   intro t x as bs h
-  rewrite [h]
-  exact (same (x :: bs))
+  rewrite [<- h]
+  exact (same (x :: as))
 
 theorem same_cons_rewrite_rfl:
   ∀ (t: Type) (x: t) (as: List t) (bs: List t),
@@ -99,9 +105,58 @@ theorem same_cons_simp_only:
 #print same_cons_simp
 #print same_cons_Implicit_Eq_subst_with_named
 
+-- What is Eq.subst and replace
+
+-- theorem Eqsubst {α : Sort u} {motive : α → Prop} {a b : α}
+--   (target : a = b) (base : motive a) : motive b :=
+-- If a Property is true for A
+-- And A = B
+-- Then that Property is true for B
+-- theorem Eqsubst {α : Sort u} {Property : α → Prop} {a b : α}
+--  (Equality : a = b) (PropertyIsTrueForA : Property a) : Property b :=
+
+-- replace target mot base
+-- replace EqualityAB Property PropertyIsTrueForA -> PropertyIsTrueForB
+
+-- Agda:
+-- subst : ∀ {A : Set} {x y : A} (P : A → Set)
+--   → x ≡ y
+--     ---------
+--   → P x → P y
+-- subst P refl px = px
+-- subst P refl base = base
+
 -- Advanced
 
+set_option pp.proofs true
+#print Eq.rec
+
+theorem Eqsubstr {α : Sort u} {motive : α → Prop} {a b : α} (target : b = a) (base : motive a) : motive b :=
+  (Eq.symm target).rec base
+
+theorem Eqsubst {α : Sort u} {motive : α → Prop} {a b : α} (target : a = b) (base : motive a) : motive b :=
+  Eqsubstr (motive := motive) (Eq.symm target) base
+
+-- recursor Eq.rec.{u, u_1} : {α : Sort u_1} →
+--   {a : α} → {motive : (a_1 : α) → a = a_1 → Sort u} → motive a (Eq.refl a) → {a_1 : α} → (t : a = a_1) → motive a_1 t
+
+theorem Eqsubst_match {α : Sort u} {motive : α → Prop} {a b : α} (target : Eq a b) (base : motive a) : motive b :=
+  match target with
+  | Eq.refl a => base
+
+@[simp] abbrev Eqndrec.{u1, u2} {α : Sort u2} {a : α} {motive : α → Sort u1} (base : motive a) {b : α} (target : Eq a b) : motive b :=
+  target.rec base
+
+theorem Eqsubst_Eqndrec {α : Sort u} {motive : α → Prop} {a b : α} (target : Eq a b) (base : motive a) : motive b :=
+  Eqndrec (motive := motive) base target
+
 #print same_cons_rewrite_rfl
+
+def Eqmpr {α β : Sort u} (h : α = β) (b : β) : α :=
+  h ▸ b
+
+def Eqmpr' {α β : Sort u} (h : α = β) (b : β) : α :=
+  (Eq.symm h).rec b
 
 theorem same_cons_mpr : ∀ (t : Type) (x : t) (as bs : List t),
   as = bs → x :: as = x :: bs :=
